src/ShouldBuild.v
@@ -63,7 +63,7 @@ From Perennial.program_proof.simplepb.simplelog Require proof.
 From Perennial.program_proof.simplepb.apps Require closed_proof kv_proof kvee_proof. *)
 
 From Perennial.program_proof.mpaxos Require
-     apply_proof.
+     applyasfollower_proof.
 
 (* MVCC *)
 From Perennial.program_proof.mvcc Require mvcc_proof.
